examples/low-level/crypto/Crypto.Symmetric.UF1CMA.fst
@@ -9,7 +9,7 @@ open FStar.HyperStack
 open FStar.Ghost
 open FStar.UInt64
 open FStar.Buffer
-open FStar.Monotonic.RRef
+//open FStar.Monotonic.RRef  // rebinding rid :(
 
 open Crypto.Symmetric.Poly1305.Spec
 open Crypto.Symmetric.Poly1305 // avoid?
@@ -26,7 +26,9 @@ module MAC = Crypto.Symmetric.MAC
 type alg = macAlg
 let alg_of_id = macAlg_of_id
 
- 
+// should go elsewhere
+let erid = r:rid{is_eternal_region r}
+
 // TOWARDS AGILITY 
 
 // length of the single-use part of the key
@@ -70,7 +72,7 @@ val akey_coerce: r:rid -> i:id -> kb: lbuffer(UInt32.v (skeylen i)) -> STL(akey 
   (requires (fun h0 -> True))
   (ensures (fun h0 r h1 -> Buffer.modifies_0 h0 h1))
 
-val akey_gen: r:rid -> i:id -> ST (akey r i)
+val akey_gen: r:erid -> i:id -> ST (akey r i)
   (requires (fun _ -> True))
   (ensures  (fun h0 k h1 ->
     if skeyed i then
@@ -85,7 +87,7 @@ let akey_gen r i =
     Some k
   else None
 
-val akey_coerce: r:rid -> i:id -> kb:lbuffer (UInt32.v (skeylen i)) -> ST (akey r i)
+val akey_coerce: r:erid -> i:id -> kb:lbuffer (UInt32.v (skeylen i)) -> ST (akey r i)
   (requires (fun h -> live h kb))
   (ensures  (fun h0 k h1 ->
     if skeyed i then
@@ -143,18 +145,20 @@ val log_cmp_transitive: a:log -> b:log -> c:log -> Lemma
   (ensures (log_cmp a b /\ log_cmp b c ==> log_cmp a c))
 let log_cmp_transitive a b c = ()
 
-val log_cmp_monotonic: unit -> Lemma (monotonic log log_cmp)
+module RR = FStar.Monotonic.RRef
+
+val log_cmp_monotonic: unit -> Lemma (RR.monotonic log log_cmp)
 let log_cmp_monotonic _ = ()
 
-let ideal_log (r:rid) = m_rref r log log_cmp
+let ideal_log (r:erid) = RR.m_rref r log log_cmp
 
-let log_ref (r:rid) = if mac_log then ideal_log r else unit
+let log_ref (r:erid) = if mac_log then ideal_log r else unit
 
-let ilog (#r:rid) (l:log_ref r{mac_log}) : Tot (ideal_log r) = l
+let ilog (#r:erid) (l:log_ref r{mac_log}) : Tot (ideal_log r) = l
 
 noeq type state (i:id) =
   | State:
-      #region: rid ->
+      #region: erid ->
       r: MAC.elemB i{Buffer.frameOf (MAC.as_buffer r) = region} -> 
       s: wordB_16 {frameOf s = region /\ disjoint (MAC.as_buffer r) s} ->
       log: log_ref region ->
@@ -163,23 +167,23 @@ noeq type state (i:id) =
 let live_ak #r (#i:id) m (ak:akey r (fst i)) = 
   skeyed (fst i) ==> live m (get_skey #r #(fst i) ak)
 
-let genPost0 (i:id) (region:rid{is_eternal_region region}) m0 (st: state i) m1 =
+let genPost0 (i:id) (region:erid) m0 (st: state i) m1 =
     ~(contains m0 (MAC.as_buffer st.r)) /\
     ~(contains m0 st.s) /\
     st.region == region /\
     MAC.norm m1 st.r /\
     Buffer.live m1 st.s /\
     (mac_log ==> 
-        ~ (m_contains (ilog st.log) m0) /\ 
-	   m_contains (ilog st.log) m1 /\ 
-	   m_sel m1 (ilog st.log) == None)
+        ~ (RR.m_contains (ilog st.log) m0) /\ 
+	   RR.m_contains (ilog st.log) m1 /\ 
+	   RR.m_sel m1 (ilog st.log) == None)
 
-let genPost (i:id) (region:rid{is_eternal_region region}) m0 (st:state i) m1 =
+let genPost (i:id) (region:erid) m0 (st:state i) m1 =
   genPost0 i region m0 st m1 /\
   modifies (Set.singleton region) m0 m1 /\
   modifies_rref region TSet.empty m0.h m1.h
 
-val alloc: region:rid{is_eternal_region region} -> i:id
+val alloc: region:erid -> i:id
   -> ak:akey region (fst i)
   -> k:lbuffer (UInt32.v (keylen (fst i)))
   -> ST (state i)
@@ -187,14 +191,13 @@ val alloc: region:rid{is_eternal_region region} -> i:id
   (ensures  (fun m0 st m1 -> genPost i region m0 st m1))
  //   (skeyed (fst i) ==> modifies_1 (get_skey #region #(fst i) st.r) m0 m1)
 
-#reset-options "--z3timeout 30 --initial_fuel 0 --max_fuel 0 --initial_ifuel 0 --max_ifuel 0"
-
+#reset-options "--z3timeout 100"
 let alloc region i sk k =
   let h0 = ST.get() in
   let r = MAC.rcreate region i in
   assert (frameOf (MAC.as_buffer r) == region);
   let s = FStar.Buffer.rcreate region 0uy 16ul in
-  cut (disjoint (MAC.as_buffer r) k /\ disjoint s k);
+  assert (disjoint (MAC.as_buffer r) k /\ disjoint s k);
   let h1 = ST.get() in
   let rb, sb =
     if skeyed (fst i) then
@@ -209,18 +212,17 @@ let alloc region i sk k =
   let h3 = ST.get() in
   lemma_reveal_modifies_1 s h2 h3;
   assume (MAC.norm h3 r);
-  assume False;
+  assume False;//16-11-27 
   if mac_log then
-    let log = m_alloc #log #log_cmp region None in
+    let log = RR.m_alloc #log #log_cmp region None in
     let h4 = ST.get() in
-    assume (MAC.norm h4 r);
+    //assume (MAC.norm h4 r);
     State #i #region r s log
   else
     State #i #region r s ()
 
-
 // for now, we require an eternal region to get monotonicity
-val gen: region:rid{is_eternal_region region} -> i:id -> ak:akey region (fst i) -> ST (state i)
+val gen: region:erid -> i:id -> ak:akey region (fst i) -> ST (state i)
   (requires (fun m0 -> live_ak m0 ak))
   (ensures (genPost i region))
 
@@ -241,7 +243,7 @@ let gen region i ak =
 //  alloc rgn i r_buff s
 
 val coerce: 
-  r:rid -> i:id{~(authId i)} -> 
+  r:erid -> i:id{~(authId i)} -> 
   ak: akey r (fst i)  -> 
   k:lbuffer (UInt32.v (keylen (fst i))) -> ST (state i)
   (requires (fun m0 -> live m0 k /\ live_ak m0 ak))
@@ -260,40 +262,58 @@ let coerce region i k0 k = alloc region i k0 k
 // we use state-passing in the spec (to be reviewed)
 // not sure what to record for separation.
 
-// should be abstract, but then we need to duplicate more elemB code
+// abstract (causing some code replication)
 
-let irtext = if mac_log then FStar.HyperStack.reference text else unit
+let irtext (r:rid) = if mac_log then (x:FStar.HyperStack.reference text{x.id = r}) else unit
 
-let mk_irtext (r:HS.reference text{mac_log}) : irtext = r
+let mk_irtext (#r:rid) (x:HS.reference text{mac_log /\ x.id = r}) : irtext r = x
 
 // 16-10-15 still missing region, needed for modifies clauses below!
 noeq abstract type accBuffer (i:id) = 
-  | Acc: a:MAC.elemB i -> l:irtext -> accBuffer i
+  | Acc: rgn:rid ->
+         a:MAC.elemB i { Buffer.frameOf (MAC.as_buffer a) = rgn } -> 
+         l:irtext rgn -> 
+         accBuffer i
 
 let alog (#i:id) (acc:accBuffer i {mac_log}): HS.reference text = acc.l
 
 let acc_inv (#i:id) (st:state i) (acc:accBuffer i) h =
-  MAC.live h st.r /\ MAC.live h acc.a /\ //not sure why I need those, implied by norm
+  //MAC.live h st.r /\ MAC.live h acc.a /\ //not sure why I need those, implied by norm
   MAC.norm h st.r /\ MAC.norm h acc.a /\ 
   disjoint (MAC.as_buffer st.r) (MAC.as_buffer acc.a) /\
   (mac_log ==> (
     let log = FStar.HyperStack.sel h (alog acc) in
     let a = MAC.sel_elem h acc.a in
     let r = MAC.sel_elem h st.r in
-    a == MAC.poly log r))
+    a == MAC.poly log r
+    ))
       
 // not framed, as we allocate private state on the caller stack
 val start: #i:id -> st:state i -> StackInline (accBuffer i)
   (requires (fun h -> MAC.norm h st.r))
   (ensures  (fun h0 a h1 -> 
+    a.rgn == h1.tip /\
     ~ (h0 `Buffer.contains` (MAC.as_buffer a.a)) /\
     acc_inv st a h1 /\ 
-    modifies_0 h0 h1))
+    (if mac_log then mods [] h0 h1 else Buffer.modifies_0 h0 h1 )))
 let start #i st =
+  let h0 = ST.get() in
+  let t : rid = h0.tip in 
   let a = MAC.start #i in
-  let l = if mac_log then mk_irtext (salloc Seq.createEmpty) else () in
-  assume False;
-  Acc a l
+  let h1 = ST.get() in 
+  lemma_reveal_modifies_0 h0 h1;
+  if mac_log then 
+    let x = salloc #text Seq.createEmpty in
+    let acc = Acc t a x in
+    let h2 = ST.get() in 
+    assert(MAC.sel_elem h1 acc.a == MAC.zero i);
+    assume(MAC.sel_elem h2 acc.a == MAC.zero i);//16-11-27 how to get framing? 
+    assert_norm(MAC.poly #i Seq.createEmpty (MAC.sel_elem h2 st.r) == MAC.zero i);
+    assert(acc_inv st acc h2); 
+    assume(mods [] h0 h2);//16-11-27  how to get transitivity? 
+    acc
+  else 
+    Acc t a ()
 
 
 // update [was add]; could add finalize (for POLY1305, last block < 16).
@@ -307,10 +327,16 @@ val update:
     // TODO. modifying both a buffer and its ref seq bytes (if present)
     // acc_modifies a h0 h1 /\  
     Buffer.live h1 w /\ 
-    acc_inv st a h1 /\ 
-    (mac_log ==> (
+    acc_inv st a h1 /\ (
+    if mac_log then (
       let v = Buffer.as_seq h1 w in
-      HS.sel h1 (alog a) == SeqProperties.cons v (HS.sel h0 (alog a))))))
+      HS.sel h1 (alog a) == SeqProperties.cons v (HS.sel h0 (alog a)))
+    else True
+      )))
+
+// mods [Ref (as_hsref (ilog st.log)); Ref (Buffer.content tag)] h0 h1 /\
+// Buffer.modifies_buf_1 (Buffer.frameOf tag) tag h0 h1 /\
+
 
 let update #i st acc w =
   //16-10-17 if mac_log then acc.l <- SeqProperties.cons w !aac.l;
@@ -335,24 +361,24 @@ val mac:
     disjoint_2 (MAC.as_buffer st.r) st.s tag /\
     disjoint st.s tag /\ 
     acc_inv st acc h0 /\
-    (mac_log ==> m_contains (ilog st.log) h0) /\
-    (mac_log /\ authId i ==> m_sel h0 (ilog st.log) == None)))
+    (mac_log ==> RR.m_contains (ilog st.log) h0) /\
+    (mac_log /\ authId i ==> RR.m_sel h0 (ilog st.log) == None)))
   (ensures (fun h0 _ h1 ->
     live h0 st.s /\ 
     live h0 (MAC.as_buffer st.r) /\ 
     live h1 tag /\
     acc_inv st acc h0 /\ (
     if mac_log then 
-      mods [Ref (as_hsref (ilog st.log)); Ref (Buffer.content tag)] h0 h1 /\
+      mods [Ref (RR.as_hsref (ilog st.log)); Ref (Buffer.content tag)] h0 h1 /\
       Buffer.modifies_buf_1 (Buffer.frameOf tag) tag h0 h1 /\
-      m_contains (ilog st.log) h1 /\ (
+      RR.m_contains (ilog st.log) h1 /\ (
       let log = FStar.HyperStack.sel h1 (alog acc) in
       let a = MAC.sel_elem h1 acc.a in
       let r = MAC.sel_elem h1 st.r in
       let s = Buffer.as_seq h1 st.s in
       let t = MAC.mac log r s in
       sel_word h1 tag === t /\
-      m_sel h1 (ilog st.log) == Some(log,t)
+      RR.m_sel h1 (ilog st.log) == Some(log,t)
       )
     else
       Buffer.modifies_1 tag h0 h1 )))
@@ -368,9 +394,9 @@ let mac #i st acc tag =
       //assume (mac_1305 l (sel_elem h0 st.r) (sel_word h0 st.s) == little_endian (sel_word h1 tag));
       let t = load_bytes 16ul tag in
       let l = !(alog acc) in
-      m_recall #st.region #log #log_cmp (ilog st.log);
-      assume (m_sel h1 (ilog st.log) == m_sel h0 (ilog st.log));
-      m_write #st.region #log #log_cmp (ilog st.log) (Some (l, t))
+      RR.m_recall #st.region #log #log_cmp (ilog st.log);
+      assume (RR.m_sel h1 (ilog st.log) == RR.m_sel h0 (ilog st.log));
+      RR.m_write #st.region #log #log_cmp (ilog st.log) (Some (l, t))
     end
   else
     admit ()
@@ -386,8 +412,8 @@ val verify:
     disjoint_2 (MAC.as_buffer acc.a) st.s tag /\ 
     disjoint_2 (MAC.as_buffer st.r) st.s tag /\
     acc_inv st acc h0 /\
-    (mac_log ==> m_contains (ilog st.log) h0) /\
-    (mac_log /\ authId i ==> is_Some (m_sel h0 (ilog st.log)))))
+    (mac_log ==> RR.m_contains (ilog st.log) h0) /\
+    (mac_log /\ authId i ==> is_Some (RR.m_sel h0 (ilog st.log)))))
         
   (ensures (fun h0 b h1 ->
     Buffer.modifies_0 h0 h1 /\
@@ -404,7 +430,7 @@ val verify:
       b = 
       ( if authId i then 
           let correct = 
-          ( match m_sel h0 (ilog st.log) with 
+          ( match RR.m_sel h0 (ilog st.log) with 
             | Some(l',m') -> m = m' && Seq.eq log l'
             | None -> false ) in
           verified && correct
